Updates due to most recent merge. Some parts of the proofs broke.

vale/code/lib/transformers/Vale.Transformers.InstructionReorder.fst
@@ -93,10 +93,9 @@ let lemma_ins_exchange_allowed_symmetric (i1 i2 : ins) :
 let equiv_states (s1 s2 : machine_state) : GTot Type0 =
   (s1.ms_ok == s2.ms_ok) /\
   (s1.ms_regs == s2.ms_regs) /\
-  (s1.ms_xmms == s2.ms_xmms) /\
   (cf s1.ms_flags = cf s2.ms_flags) /\
   (overflow s1.ms_flags = overflow s2.ms_flags) /\
-  (s1.ms_mem == s2.ms_mem) /\
+  (s1.ms_heap == s2.ms_heap) /\
   (s1.ms_memTaint == s2.ms_memTaint) /\
   (s1.ms_stack == s2.ms_stack) /\
   (s1.ms_stackTaint == s2.ms_stackTaint)
@@ -106,8 +105,7 @@ let equiv_states (s1 s2 : machine_state) : GTot Type0 =
 let equiv_states_ext (s1 s2 : machine_state) : GTot Type0 =
   let open FStar.FunctionalExtensionality in
   (feq s1.ms_regs s2.ms_regs) /\
-  (feq s1.ms_xmms s2.ms_xmms) /\
-  (Map.equal s1.ms_mem s2.ms_mem) /\
+  (Map.equal s1.ms_heap s2.ms_heap) /\
   (Map.equal s1.ms_memTaint s2.ms_memTaint) /\
   (Map.equal s1.ms_stack.stack_mem s2.ms_stack.stack_mem) /\
   (Map.equal s1.ms_stackTaint s2.ms_stackTaint) /\
@@ -270,19 +268,19 @@ let lemma_eval_instr_equiv_states
         equiv_ostates
           (eval_instr it oprs ann s1)
           (eval_instr it oprs ann s2))) =
-  let InstrTypeRecord #outs #args #havoc_flags i = it in
+  let InstrTypeRecord #outs #args #havoc_flags' i = it in
   let vs1 = instr_apply_eval outs args (instr_eval i) oprs s1 in
   let vs2 = instr_apply_eval outs args (instr_eval i) oprs s2 in
   lemma_instr_apply_eval_inouts_equiv_states outs outs args (instr_eval i) oprs s1 s2;
   assert (vs1 == vs2);
   let s1_new =
-    match havoc_flags with
-    | HavocFlags -> {s1 with ms_flags = havoc_state_ins s1 (Instr it oprs ann)}
+    match havoc_flags' with
+    | HavocFlags -> {s1 with ms_flags = havoc_flags}
     | PreserveFlags -> s1
   in
   let s2_new =
-    match havoc_flags with
-    | HavocFlags -> {s2 with ms_flags = havoc_state_ins s2 (Instr it oprs ann)}
+    match havoc_flags' with
+    | HavocFlags -> {s2 with ms_flags = havoc_flags}
     | PreserveFlags -> s2
   in
   assume (overflow s1_new.ms_flags == overflow s2_new.ms_flags); (* TODO FIXME *)
@@ -300,34 +298,36 @@ let lemma_eval_instr_equiv_states
    TODO: Figure out why it is slowing down so much. It practically
          brings F* to a standstill even when editing, and it acts
          worse during an interactive proof. *)
-let lemma_untainted_eval_ins_equiv_states (i : ins) (s1 s2 : machine_state) :
+let lemma_machine_eval_ins_st_equiv_states (i : ins) (s1 s2 : machine_state) :
   Lemma
     (requires (equiv_states s1 s2))
     (ensures (
         equiv_states
-          (run (untainted_eval_ins i) s1)
-          (run (untainted_eval_ins i) s2))) =
+          (run (machine_eval_ins_st i) s1)
+          (run (machine_eval_ins_st i) s2))) =
   let s1_orig, s2_orig = s1, s2 in
-  let s1_final = run (untainted_eval_ins i) s1 in
-  let s2_final = run (untainted_eval_ins i) s2 in
+  let s1_final = run (machine_eval_ins_st i) s1 in
+  let s2_final = run (machine_eval_ins_st i) s2 in
   match i with
   | Instr it oprs ann ->
     lemma_eval_instr_equiv_states it oprs ann s1 s2
   | Push _ _ ->
+    admit (); (* TODO FIXME: Broke during merge with fstar-master *)
     assert_spinoff (equiv_states_ext s1_final s2_final)
   | Pop dst t ->
-    let stack_op = OStack (MReg rRsp 0, t) in
+    admit (); (* TODO FIXME: Broke during merge with fstar-master *)
+    let stack_op = OStack (MReg (Reg 0 rRsp) 0, t) in
     let s1 = proof_run s1 (check (valid_src_operand stack_op)) in
     let s2 = proof_run s2 (check (valid_src_operand stack_op)) in
     // assert (equiv_states s1 s2);
     let new_dst1 = eval_operand stack_op s1 in
     let new_dst2 = eval_operand stack_op s2 in
     // assert (new_dst1 == new_dst2);
-    let new_rsp1 = (eval_reg rRsp s1 + 8) % pow2_64 in
-    let new_rsp2 = (eval_reg rRsp s2 + 8) % pow2_64 in
+    let new_rsp1 = (eval_reg_64 rRsp s1 + 8) % pow2_64 in
+    let new_rsp2 = (eval_reg_64 rRsp s2 + 8) % pow2_64 in
     // assert (new_rsp1 == new_rsp2);
-    let s1 = proof_run s1 (update_operand_preserve_flags dst new_dst1) in
-    let s2 = proof_run s2 (update_operand_preserve_flags dst new_dst2) in
+    let s1 = proof_run s1 (update_operand64_preserve_flags dst new_dst1) in
+    let s2 = proof_run s2 (update_operand64_preserve_flags dst new_dst2) in
     assert (equiv_states_ext s1 s2);
     let s1 = proof_run s1 (free_stack (new_rsp1 - 8) new_rsp1) in
     let s2 = proof_run s2 (free_stack (new_rsp2 - 8) new_rsp2) in
@@ -341,107 +341,6 @@ let lemma_untainted_eval_ins_equiv_states (i : ins) (s1 s2 : machine_state) :
   | Dealloc _ ->
     assert_spinoff (equiv_states_ext s1_final s2_final)
 
-let rec lemma_taint_match_args_equiv_states
-    (args:list instr_operand)
-    (oprs:instr_operands_t_args args)
-    (memTaint:memTaint_t)
-    (stackTaint:memTaint_t)
-    (s1 s2:machine_state) :
-  Lemma
-    (requires (equiv_states s1 s2))
-    (ensures (
-        (taint_match_args args oprs memTaint stackTaint s1) ==
-        (taint_match_args args oprs memTaint stackTaint s2))) =
-  match args with
-  | [] -> ()
-  | i :: args ->
-    match i with
-    | IOpEx i ->
-      let oprs : instr_operand_t i & instr_operands_t_args args = coerce oprs in
-      lemma_taint_match_args_equiv_states args (snd oprs) memTaint stackTaint s1 s2
-    | IOpIm i ->
-      lemma_taint_match_args_equiv_states args (coerce oprs) memTaint stackTaint s1 s2
-
-let rec lemma_taint_match_inouts_equiv_states
-    (inouts:list instr_out)
-    (args:list instr_operand)
-    (oprs:instr_operands_t inouts args)
-    (memTaint:memTaint_t)
-    (stackTaint:memTaint_t)
-    (s1 s2:machine_state) :
-  Lemma
-    (requires (equiv_states s1 s2))
-    (ensures (
-        (taint_match_inouts inouts args oprs memTaint stackTaint s1) ==
-        (taint_match_inouts inouts args oprs memTaint stackTaint s2))) =
-  match inouts with
-  | [] -> lemma_taint_match_args_equiv_states args oprs memTaint stackTaint s1 s2
-  | (Out, i) :: inouts ->
-    let oprs =
-      match i with
-      | IOpEx i -> snd #(instr_operand_t i) (coerce oprs)
-      | IOpIm i -> coerce oprs
-    in
-    lemma_taint_match_inouts_equiv_states inouts args oprs memTaint stackTaint s1 s2
-  | (InOut, i)::inouts ->
-    let (v, oprs) =
-      match i with
-      | IOpEx i ->
-        let oprs = coerce oprs in
-        (taint_match_operand_explicit i (fst oprs) memTaint stackTaint s1, snd oprs)
-      | IOpIm i -> (taint_match_operand_implicit i memTaint stackTaint s1, coerce oprs)
-    in
-    lemma_taint_match_inouts_equiv_states inouts args oprs memTaint stackTaint s1 s2
-
-let lemma_taint_match_ins_equiv_states (i : ins) (s1 s2 : machine_state) :
-  Lemma
-    (requires (equiv_states s1 s2))
-    (ensures (
-        (taint_match_ins i s1.ms_memTaint s1.ms_stackTaint s1) ==
-        (taint_match_ins i s2.ms_memTaint s2.ms_stackTaint s2))) =
-  match i with
-  | Instr (InstrTypeRecord #outs #args _) oprs _ ->
-    assert (s1.ms_memTaint == s2.ms_memTaint);
-    assert (s1.ms_stackTaint == s2.ms_stackTaint);
-    lemma_taint_match_inouts_equiv_states outs args oprs s1.ms_memTaint s1.ms_stackTaint s1 s2
-  | Push _ _ | Pop _ _ | Alloc _ | Dealloc _ -> ()
-
-let rec lemma_update_taint_outputs_equiv_states
-    (outs:list instr_out) (args:list instr_operand) (oprs:instr_operands_t outs args)
-    (memTaint:memTaint_t) (stackTaint:memTaint_t)
-    (s1 s2:machine_state) :
-  Lemma
-    (requires (equiv_states s1 s2))
-    (ensures (
-        (update_taint_outputs outs args oprs memTaint stackTaint s1) ==
-        (update_taint_outputs outs args oprs memTaint stackTaint s2))) =
-  match outs with
-  | [] -> ()
-  | (_, i) :: outs ->
-    let ((memTaint, stackTaint), oprs) =
-      match i with
-      | IOpEx i ->
-        let oprs = coerce oprs in
-        (update_taint_operand_explicit i (fst oprs) memTaint stackTaint s1, snd oprs)
-      | IOpIm i -> (update_taint_operand_implicit i memTaint stackTaint s1, coerce oprs)
-    in
-    lemma_update_taint_outputs_equiv_states outs args oprs memTaint stackTaint s1 s2
-
-let lemma_update_taint_ins_equiv_states
-    (i : ins)
-    (memTaint:memTaint_t)
-    (stackTaint:memTaint_t)
-    (s1 s2:machine_state) :
-  Lemma
-    (requires (equiv_states s1 s2))
-    (ensures (
-        (update_taint_ins i memTaint stackTaint s1) ==
-        (update_taint_ins i memTaint stackTaint s2))) =
-  match i with
-  | Instr (InstrTypeRecord #outs #args _) oprs _ ->
-    lemma_update_taint_outputs_equiv_states outs args oprs memTaint stackTaint s1 s2
-  | Push _ _ | Pop _ _ | Alloc _ | Dealloc _ -> ()
-
 let lemma_eval_ins_equiv_states (i : ins) (s1 s2 : machine_state) :
   Lemma
     (requires (equiv_states s1 s2))
@@ -449,21 +348,7 @@ let lemma_eval_ins_equiv_states (i : ins) (s1 s2 : machine_state) :
         equiv_states
           (machine_eval_ins i s1)
           (machine_eval_ins i s2))) =
-  let s10 = run (check (taint_match_ins i s1.ms_memTaint s1.ms_stackTaint)) s1 in
-  let s20 = run (check (taint_match_ins i s2.ms_memTaint s2.ms_stackTaint)) s2 in
-  lemma_taint_match_ins_equiv_states i s1 s2;
-  assert (equiv_states s10 s20);
-  let memTaint1, stackTaint1 = update_taint_ins i s1.ms_memTaint s1.ms_stackTaint s10 in
-  let memTaint2, stackTaint2 = update_taint_ins i s2.ms_memTaint s2.ms_stackTaint s20 in
-  lemma_update_taint_ins_equiv_states i s1.ms_memTaint s2.ms_stackTaint s10 s20;
-  assert (memTaint1 == memTaint2);
-  assert (stackTaint1 == stackTaint2);
-  let s11 = run (untainted_eval_ins i) s10 in
-  let s21 = run (untainted_eval_ins i) s20 in
-  lemma_untainted_eval_ins_equiv_states i s10 s20;
-  let s12 = { s11 with ms_memTaint = memTaint1 ; ms_stackTaint = stackTaint1 } in
-  let s22 = { s21 with ms_memTaint = memTaint2 ; ms_stackTaint = stackTaint2 } in
-  assert (equiv_states s12 s22)
+  lemma_machine_eval_ins_st_equiv_states i s1 s2
 
 (** Filter out observation related stuff from the state. *)
 let filt_state (s:machine_state) =
@@ -862,51 +747,51 @@ let lemma_commute (f1 f2:st unit) (r1 w1 r2 w2:list location) (s:machine_state) 
   lemma_equiv_states_when_except_none is12 is21 s12.ms_ok;
   assert (equiv_states (run2 f1 f2 s) (run2 f2 f1 s))
 
-let lemma_untainted_eval_ins_only_affects_write_aux (i:ins{Instr? i}) (s:machine_state) (a:location) :
+let lemma_machine_eval_ins_st_only_affects_write_aux (i:ins{Instr? i}) (s:machine_state) (a:location) :
   Lemma
     (requires (
         let r, w = rw_set_of_ins i in
         (!!(disjoint_location_from_locations a w))))
     (ensures (
-        (eval_location a s == eval_location a (run (untainted_eval_ins i) s)))) =
+        (eval_location a s == eval_location a (run (machine_eval_ins_st i) s)))) =
   admit ()
 
-let lemma_untainted_eval_ins_only_affects_write (i:ins{Instr? i}) (s:machine_state) :
+let lemma_machine_eval_ins_st_only_affects_write (i:ins{Instr? i}) (s:machine_state) :
   Lemma
     (ensures (
        (let r, w = rw_set_of_ins i in
-        (unchanged_except w s (run (untainted_eval_ins i) s))))) =
+        (unchanged_except w s (run (machine_eval_ins_st i) s))))) =
   FStar.Classical.forall_intro (
-    FStar.Classical.move_requires (lemma_untainted_eval_ins_only_affects_write_aux i s))
+    FStar.Classical.move_requires (lemma_machine_eval_ins_st_only_affects_write_aux i s))
 
-let lemma_untainted_eval_ins_unchanged_behavior (i:ins{Instr? i}) (s1 s2:machine_state) :
+let lemma_machine_eval_ins_st_unchanged_behavior (i:ins{Instr? i}) (s1 s2:machine_state) :
   Lemma
     (requires (
         let r, w = rw_set_of_ins i in
         (unchanged_at r s1 s2)))
     (ensures (
         let r, w = rw_set_of_ins i in
-        let f = untainted_eval_ins i in
+        let f = machine_eval_ins_st i in
         (unchanged_at w (run f s1) (run f s2)) /\
         (run f s1).ms_ok = (run f s2).ms_ok)) =
   admit ()
 
-let lemma_untainted_eval_ins_bounded_effects (i:ins{Instr? i}) :
+let lemma_machine_eval_ins_st_bounded_effects (i:ins{Instr? i}) :
   Lemma
     (ensures (
         (let r, w = rw_set_of_ins i in
-         (bounded_effects r w (untainted_eval_ins i))))) =
-  FStar.Classical.forall_intro (lemma_untainted_eval_ins_only_affects_write i);
+         (bounded_effects r w (machine_eval_ins_st i))))) =
+  FStar.Classical.forall_intro (lemma_machine_eval_ins_st_only_affects_write i);
   FStar.Classical.forall_intro_2 (fun s1 ->
-      FStar.Classical.move_requires (lemma_untainted_eval_ins_unchanged_behavior i s1))
+      FStar.Classical.move_requires (lemma_machine_eval_ins_st_unchanged_behavior i s1))
 
-let lemma_untainted_eval_ins_exchange (i1 i2 : ins) (s : machine_state) :
+let lemma_machine_eval_ins_st_exchange (i1 i2 : ins) (s : machine_state) :
   Lemma
     (requires (!!(ins_exchange_allowed i1 i2)))
     (ensures (commutes s
-                (untainted_eval_ins i1)
-                (untainted_eval_ins i2))) =
-  let f = untainted_eval_ins i1 in
+                (machine_eval_ins_st i1)
+                (machine_eval_ins_st i2))) =
+  let f = machine_eval_ins_st i1 in
   match i2 with
   | Instr it oprs ann ->
     admit ()
@@ -985,6 +870,7 @@ let lemma_code_exchange (c1 c2 : code) (fuel:nat) (s1 s2 : machine_state) :
     machine_eval_codes [c2; c1] fuel s2 in
   match c1, c2 with
   | Ins i1, Ins i2 ->
+    admit (); (* TODO FIXME: Broke during merge with fstar-master *)
     let Some s10 = machine_eval_code c1 fuel s1 in
     let Some s11 = machine_eval_code c1 fuel (filt_state s1) in
     // assert_norm (equiv_states s10 s11);
